Update tests

tests/lean/run/issue2237.lean
@@ -12,11 +12,22 @@ inductive Term : Context → Ty → Type where
 | lam : Term (✶ :: Γ) ✶ → Term Γ ✶
 | ap : Term Γ ✶ → Term Γ ✶ → Term Γ ✶
 
+-- set_option trace.Meta.Match.matchEqs true
+
 abbrev plus : Term Γ a → Term Γ a
 | .var i => .var i
 | .lam n => .lam (plus n)
 | .ap (.lam _) m => plus m -- This case takes precedence over the next one.
 | .ap l m => (plus l).ap (plus m)
+
+/--
+info: plus.match_1.{u_1} {Γ : Context} {a : Ty} (motive : Term Γ a → Sort u_1) (x✝ : Term Γ a)
+  (h_1 : (i : Lookup Γ a) → motive (Term.var i)) (h_2 : (n : Term ( ✶ :: Γ) ✶ ) → motive n.lam)
+  (h_3 : (a : Term ( ✶ :: Γ) ✶ ) → (m : Term Γ ✶ ) → motive (a.lam.ap m)) (h_4 : (l m : Term Γ ✶ ) → motive (l.ap m)) :
+  motive x✝
+-/
+#guard_msgs(pass trace, all) in
+#check plus.match_1
 
 /--
 error: failed to generate equational theorem for `plus`
@@ -29,7 +40,7 @@ error: failed to generate equational theorem for `plus`
   in the application
     @HEq (Term Γ a) (l.ap m)
 -/
-#guard_msgs in
+#guard_msgs(pass trace, all) in
 #print equations plus
 
 
@@ -46,7 +57,8 @@ error: Failed to realize constant plus.match_1.eq_1:
 ---
 error: Unknown constant `plus.match_1.eq_1`
 -/
-#guard_msgs in #print sig plus.match_1.eq_1
+#guard_msgs(pass trace, all) in
+#print sig plus.match_1.eq_1
 
 /--
 error: Failed to realize constant plus.match_1.congr_eq_1:
@@ -62,4 +74,44 @@ error: Failed to realize constant plus.match_1.congr_eq_1:
 ---
 error: Unknown constant `plus.match_1.congr_eq_1`
 -/
-#guard_msgs in #print sig plus.match_1.congr_eq_1
+#guard_msgs(pass trace, all) in
+#print sig plus.match_1.congr_eq_1
+
+-- Work-around: include the index in pattern matching directly
+
+def plus' (t : Term Γ a) : Term Γ a := match a, t with
+| _, .var i => .var i
+| _, .lam n => .lam (plus n)
+| _, .ap (.lam _) m => plus m -- This case takes precedence over the next one.
+| _, .ap l m => (plus l).ap (plus m)
+
+/--
+info: equations:
+@[defeq] theorem plus'.eq_1 : ∀ {Γ : Context} {a : Ty} (i : Lookup Γ a), plus' (Term.var i) = Term.var i
+@[defeq] theorem plus'.eq_2 : ∀ {Γ : Context} (n : Term ( ✶ :: Γ) ✶ ), plus' n.lam = (plus n).lam
+@[defeq] theorem plus'.eq_3 : ∀ {Γ : Context} (a_2 : Term ( ✶ :: Γ) ✶ ) (m : Term Γ ✶ ), plus' (a_2.lam.ap m) = plus m
+theorem plus'.eq_4 : ∀ {Γ : Context} (l m : Term Γ ✶ ),
+  (∀ (a : Term ( ✶ :: Γ) ✶ ), l = a.lam → False) → plus' (l.ap m) = (plus l).ap (plus m)
+-/
+#guard_msgs(pass trace, all) in
+#print equations plus'
+
+
+/--
+info: private theorem plus'.match_1.congr_eq_4.{u_1} : ∀ {Γ : Context} (motive : (a : Ty) → Term Γ a → Sort u_1) (a : Ty)
+  (t : Term Γ a) (h_1 : (x : Ty) → (i : Lookup Γ x) → motive x (Term.var i))
+  (h_2 : (n : Term ( ✶ :: Γ) ✶ ) → motive ✶ n.lam)
+  (h_3 : (a : Term ( ✶ :: Γ) ✶ ) → (m : Term Γ ✶ ) → motive ✶ (a.lam.ap m))
+  (h_4 : (l m : Term Γ ✶ ) → motive ✶ (l.ap m)) (l m : Term Γ ✶ ),
+  a = ✶ →
+    t ≍ l.ap m →
+      (∀ (a : Term ( ✶ :: Γ) ✶ ) (m_1 : Term Γ ✶ ), ✶ = ✶ → l.ap m ≍ a.lam.ap m_1 → False) →
+        (match a, t with
+          | x, Term.var i => h_1 x i
+          | .( ✶ ), n.lam => h_2 n
+          | .( ✶ ), a.lam.ap m => h_3 a m
+          | .( ✶ ), l.ap m => h_4 l m) ≍
+          h_4 l m
+-/
+#guard_msgs(pass trace, all) in
+#print sig plus'.match_1.congr_eq_4
